src/dvc_implementation/block_proposer/block_dvc_externs.dfy
@@ -1,6 +1,5 @@
 include "../../common/commons.dfy"
-include "../../common/commons.dfy"
-include "../../common/block_proposer/block_signing_functions.dfy"
+
 
 module Block_DVC_Externs
 {
