src/proofs/implementation_refinement/attestation_creation/dvc_spec_spec_instr_on_blocks_refinement.dfy
@@ -1,6 +1,3 @@
-include "../../../common/commons.dfy"
-include "../../../common/commons.dfy"
-
 include "../../../proofs/no_slashable_blocks/common/block_dvc_spec_axioms.dfy"
 include "../../../proofs/no_slashable_blocks/common/dvc_block_proposer_instrumented.dfy"
 include "../../../specs/dvc/dvc_block_proposer.dfy"
