src/proofs/no_slashable_blocks/common/common_proofs.dfy
@@ -1,9 +1,8 @@
 include "../../../common/commons.dfy"
-include "../../../common/commons.dfy"
 
 include "dvc_block_proposer_instrumented.dfy"
 include "../../../specs/consensus/block_consensus.dfy"
-include "../../../specs/network/block_network.dfy"
+include "../../../specs/network/network.dfy"
 include "../supporting_lemmas/inv.dfy"
 include "../../common/helper_sets_lemmas.dfy"
 include "block_dvc_spec_axioms.dfy"
@@ -14,7 +13,7 @@ module Common_Proofs_For_Block_Proposer
     import opened Types 
     import opened CommonFunctions
     import opened Block_Consensus_Spec
-    import opened Block_Network_Spec
+    import opened NetworkSpec
     import opened DVC_Block_Proposer_Spec_Instr
     import opened DV_Block_Proposer_Spec
     import opened Block_Inv_With_Empty_Initial_Block_Slashing_DB
