src/proofs/no_slashable_blocks/supporting_lemmas/dv_next_preserves_ind_inv/ind_inv_dv_next.dfy
@@ -1,11 +1,10 @@
 include "../../../../common/commons.dfy"
-include "../../../../common/commons.dfy"
-include "../../../../common/block_proposer/block_signing_functions.dfy"
+
 include "../../common/dvc_block_proposer_instrumented.dfy"
 include "../../common/block_dvc_spec_axioms.dfy"
 
 include "../../../../specs/consensus/block_consensus.dfy"
-include "../../../../specs/network/block_network.dfy"
+include "../../../../specs/network/network.dfy"
 include "../../../../specs/dv/dv_block_proposer.dfy"
 
 include "invs_fnc_1.dfy"
@@ -27,7 +26,7 @@ module Ind_Inv_DV_Next
     
     import opened CommonFunctions
     import opened Block_Consensus_Spec
-    import opened Block_Network_Spec
+    import opened NetworkSpec
     import opened DVC_Block_Proposer_Spec_Instr
     import opened DVC_Block_Proposer_Spec_Axioms
     import opened Block_Inv_With_Empty_Initial_Block_Slashing_DB
