src/proofs/no_slashable_blocks/supporting_lemmas/dv_next_preserves_ind_inv/invs_dv_next_4.dfy
@@ -2,13 +2,12 @@ include "../../../../common/commons.dfy"
 include "invs_fnc_1.dfy"
 include "invs_fnc_2.dfy"
 
-include "../../../../common/commons.dfy"
-include "../../../../common/block_proposer/block_signing_functions.dfy"
+
 include "../../common/dvc_block_proposer_instrumented.dfy"
 include "../../common/block_dvc_spec_axioms.dfy"
 
 include "../../../../specs/consensus/block_consensus.dfy"
-include "../../../../specs/network/block_network.dfy"
+include "../../../../specs/network/network.dfy"
 include "../../../../specs/dv/dv_block_proposer.dfy"
 include "../inv.dfy"
 
@@ -31,7 +30,7 @@ module Invs_DV_Next_4
     
     import opened CommonFunctions
     import opened Block_Consensus_Spec
-    import opened Block_Network_Spec
+    import opened NetworkSpec
     import opened DVC_Block_Proposer_Spec_Instr
     import opened DVC_Block_Proposer_Spec_Axioms
     import opened Block_Inv_With_Empty_Initial_Block_Slashing_DB
@@ -128,7 +127,7 @@ module Invs_DV_Next_4
         var dvc := dv.honest_nodes_states[node];
         var dvc' := dv'.honest_nodes_states[node];
                 
-        assert Block_Network_Spec.Next(dv.block_share_network, dv'.block_share_network, node, nodeOutputs.sent_block_shares, {block_share});
+        assert NetworkSpec.Next(dv.block_share_network, dv'.block_share_network, node, nodeOutputs.sent_block_shares, {block_share});
         assert multiset(addReceipientToMessages<SignedBeaconBlock>({block_share}, node)) <= dv.block_share_network.messagesInTransit;
         assert MessaageWithRecipient(message := block_share, receipient := node) in dv.block_share_network.messagesInTransit;        
         assert block_share in dv.block_share_network.allMessagesSent;
