src/proofs/no_slashable_blocks/supporting_lemmas/inv.dfy
@@ -1,8 +1,7 @@
 include "../../../common/commons.dfy"
-include "../../../common/commons.dfy"
 
 include "../../../specs/consensus/block_consensus.dfy"
-include "../../../specs/network/block_network.dfy"
+include "../../../specs/network/network.dfy"
 include "../../../specs/dv/dv_block_proposer.dfy"
 include "../common/dvc_block_proposer_instrumented.dfy"
 include "../../common/helper_sets_lemmas.dfy"
@@ -16,7 +15,7 @@ module Block_Inv_With_Empty_Initial_Block_Slashing_DB
     import opened CommonFunctions
     
     import opened Block_Consensus_Spec
-    import opened Block_Network_Spec
+    import opened NetworkSpec
     import opened DVC_Block_Proposer_Spec_Instr
     import opened DV_Block_Proposer_Spec
     import opened Helper_Sets_Lemmas
